src/SemFacts.v
@@ -1,6 +1,44 @@
 Require Import Bool List String Peano_dec.
 Require Import Common FMap Syntax Semantics.
 
+Lemma steps_split:
+  forall {MsgT} (step: Step MsgT) sys st1 st2 ll,
+    steps step sys st1 ll st2 ->
+    forall ll1 ll2,
+      ll = ll2 ++ ll1 ->
+      exists sti,
+        steps step sys st1 ll1 sti /\
+        steps step sys sti ll2 st2.
+Proof.
+  induction 1; simpl; intros.
+  - apply eq_sym, app_eq_nil in H; dest; subst.
+    eexists; split; econstructor.
+  - destruct ll2.
+    + simpl in H1; subst.
+      specialize (IHsteps ll nil eq_refl).
+      destruct IHsteps as [sti [? ?]].
+      inv H2.
+      eexists; split.
+      * econstructor; eauto.
+      * econstructor.
+    + simpl in H1; inv H1.
+      specialize (IHsteps _ _ eq_refl).
+      destruct IHsteps as [sti [? ?]].
+      eexists; split; eauto.
+      econstructor; eauto.
+Qed.
+
+Lemma steps_append:
+  forall {MsgT} (step: Step MsgT) sys st1 ll1 st2,
+    steps step sys st1 ll1 st2 ->
+    forall ll2 st3,
+      steps step sys st2 ll2 st3 ->
+      steps step sys st1 (ll2 ++ ll1) st3.
+Proof.
+  induction 2; simpl; intros; [auto|].
+  econstructor; eauto.
+Qed.
+
 Theorem refines_refl:
   forall (step: Step Msg) sys, step # step |-- sys ⊑[id] sys.
 Proof.
